PAC_Checker/Aux_Lemmas.thy
@@ -1,0 +1,74 @@
+theory Aux_Lemmas
+  imports Main Isabelle_LLVM.IICF
+begin
+
+text \<open>Lemmas and Definitions that are not available in Isabelle LLVM, but where
+(possibly indirectly) available in Refine_Imperative HOL\<close>
+
+text \<open>From Separation_Logic_Imperative_HOL.Hash_Map\<close>
+lemma take_set: "set (take n l) = { l!i | i. i<n \<and> i<length l }"
+  apply (auto simp add: set_conv_nth)
+  apply (rule_tac x=i in exI)
+  apply auto
+  done
+
+text \<open>From Refine_Imperative_HOL.IICF_List_Mset\<close>
+definition "list_mset_rel \<equiv> br mset (\<lambda>_. True)"
+
+text \<open>From Refine_Imperative_HOL.Sepref_Foreach\<close>
+definition "monadic_nfoldli l c f s \<equiv> RECT (\<lambda>D (l,s). case l of 
+    [] \<Rightarrow> RETURN s
+  | x#ls \<Rightarrow> do {
+      b \<leftarrow> c s;
+      if b then do { s'\<leftarrow>f x s; D (ls,s')} else RETURN s
+    }
+  ) (l,s)"
+
+lemma monadic_nfoldli_eq:
+  "monadic_nfoldli l c f s = (
+    case l of 
+      [] \<Rightarrow> RETURN s 
+    | x#ls \<Rightarrow> do {
+        b\<leftarrow>c s; 
+        if b then f x s \<bind> monadic_nfoldli ls c f else RETURN s
+      }
+  )"
+  apply (subst monadic_nfoldli_def)
+  apply (subst RECT_unfold)
+  apply (tagged_solver)
+  apply (subst monadic_nfoldli_def[symmetric])
+  apply simp
+  done
+
+lemma monadic_nfoldli_simp[simp]:
+  "monadic_nfoldli [] c f s = RETURN s"
+  "monadic_nfoldli (x#ls) c f s = do {
+    b\<leftarrow>c s;
+    if b then f x s \<bind> monadic_nfoldli ls c f else RETURN s
+  }"
+  apply (subst monadic_nfoldli_eq, simp)
+  apply (subst monadic_nfoldli_eq, simp)
+  done
+
+text \<open>Does not exist. Note that we have to properly implement Hashmaps\<close>
+
+(* type of hm.assn (with refine imperative)
+\<open>"('c \<Rightarrow> 'a \<Rightarrow> assn) \<Rightarrow> ('d \<Rightarrow> 'b \<Rightarrow> assn) \<Rightarrow> ('c \<Rightarrow> 'd option) \<Rightarrow> ('a, 'b) hashtable \<Rightarrow> assn"\<close>
+*)
+
+(* type of hr_comp (with refine imperative)
+"hr_comp"
+:: "('a \<Rightarrow> 'b \<Rightarrow> assn) \<Rightarrow> ('a \<times> 'c) set \<Rightarrow> 'c \<Rightarrow> 'b \<Rightarrow> assn"
+*)
+
+(* type of hr_comp (with isabelle llvm backend)
+"hr_comp"
+  :: "('a \<Rightarrow> 'b \<Rightarrow> llvm_amemory \<Rightarrow> bool) \<Rightarrow> ('a \<times> 'c) set \<Rightarrow> 'c \<Rightarrow> 'b \<Rightarrow> llvm_amemory \<Rightarrow> bool"
+*)
+(* Note assn = (llvm_amemory \<Rightarrow> bool) ind isabelle llvm*)
+
+(* So hm_assn (for isabelle llvm backend) should have type
+... llvm_amemory \<Rightarrow> bool
+*)
+
+end
