PAC_Checker/String_Array_Assn.thy
@@ -1,0 +1,7 @@
+theory String_Array_Assn
+  imports Char_Assn
+begin
+
+definition \<open>string_assn \<equiv> larray_assn' TYPE(64) char_assn\<close>
+
+end
